Tables/Table/Raw.lean
@@ -1,0 +1,6 @@
+module
+
+public import Tables.Table.Raw.Basic
+public import Tables.Table.Raw.BasicLemmas
+public import Tables.Table.Raw.Join
+public import Tables.Table.Raw.JoinLemmas
