Tables/Table/Raw/JoinLemmas.lean
@@ -26,4 +26,26 @@ theorem wfColumnSize_leftJoin (self other : Raw) (keys : Array String)
 
 end wfColumnSize
 
+section schema
+
+theorem distinct_schema (self : Raw) (h : self.WfColumnSize) :
+    (distinct self h).schema = self.schema := by
+  unfold distinct
+  apply ofRows_schema
+
+theorem crossJoin_schema (self other : Raw) (h₁ : self.WfColumnSize) (h₂ : other.WfColumnSize) :
+    (crossJoin self other h₁ h₂).schema = self.schema ++ other.schema := by
+  unfold crossJoin
+  apply ofRows_schema
+
+theorem leftJoin_schema (self other : Raw) (keys : Array String)
+    (h₁ : self.WfColumnSize) (h₂ : other.WfColumnSize) :
+    (leftJoin self other keys h₁ h₂).schema = self.schema ++ other.schema.selectNotByNames keys := by
+  unfold leftJoin
+  apply ofRows_schema
+
+end schema
+
 end Tables.Table.Raw
+
+end
